Support exceptions in monadic implementation (#17)

cluster/isabelle/Monadic.thy
@@ -2,34 +2,43 @@ theory Monadic
   imports Implementation "~~/src/HOL/Library/Monad_Syntax"
 begin
 
-datatype 'a Action = Action "NodeData \<Rightarrow> (NodeData * RoutedMessage list * 'a)"
+datatype Exception = IllegalArgumentException
 
-definition return :: "'a \<Rightarrow> 'a Action" where "return a \<equiv> Action (\<lambda> nd. (nd, [], a))"
+datatype ('e,'a) Result = Success 'a | Exception 'e
+
+datatype 'a Action = Action "NodeData \<Rightarrow> (NodeData * RoutedMessage list * (Exception,'a) Result)"
+
+definition runM :: "'a Action \<Rightarrow> NodeData \<Rightarrow> (NodeData * RoutedMessage list * (Exception,'a) Result)"
+  where "runM ma \<equiv> case ma of Action unwrapped_ma \<Rightarrow> unwrapped_ma"
+
+lemma runM_Action[simp]: "runM (Action f) = f" by (simp add: runM_def)
+lemma runM_inject[intro]: "(\<And>nd. runM ma nd = runM mb nd) \<Longrightarrow> ma = mb" by (cases ma, cases mb, auto simp add: runM_def)
+
+definition return :: "'a \<Rightarrow> 'a Action" where "return a \<equiv> Action (\<lambda> nd. (nd, [], Success a))"
+
+lemma runM_return[simp]: "runM (return a) nd = (nd, [], Success a)" unfolding runM_def return_def by simp
 
 definition Action_bind :: "'a Action \<Rightarrow> ('a \<Rightarrow> 'b Action) \<Rightarrow> 'b Action"
-  where "Action_bind ma mf \<equiv> case ma of
-    Action unwrapped_ma \<Rightarrow> Action (\<lambda> nd0. case unwrapped_ma nd0 of
-      (nd1, msgs0, a) \<Rightarrow> case mf a of
-        Action unwrapped_mb \<Rightarrow> case unwrapped_mb nd1 of
-          (nd2, msgs1, b) \<Rightarrow> (nd2, msgs0 @ msgs1, b))"
+  where "Action_bind ma mf \<equiv> Action (\<lambda> nd0. case runM ma nd0 of
+      (nd1, msgs1, result1) \<Rightarrow> (case result1 of
+          Exception e \<Rightarrow> (nd1, msgs1, Exception e)
+        | Success a \<Rightarrow> (case runM (mf a) nd1 of
+             (nd2, msgs2, result2) \<Rightarrow> (nd2, msgs1 @ msgs2, result2))))"
 
 adhoc_overloading bind Action_bind
 
-definition runM :: "'a Action \<Rightarrow> NodeData \<Rightarrow> (NodeData * RoutedMessage list * 'a)"
-  where "runM ma \<equiv> case ma of Action unwrapped_ma \<Rightarrow> unwrapped_ma"
-
-lemma runM_action[simp]: "runM (Action f) = f" by (simp add: runM_def)
-lemma runM_inject[intro]: "(\<And>nd. runM ma nd = runM mb nd) \<Longrightarrow> ma = mb" by (cases ma, cases mb, auto simp add: runM_def)
-
-lemma runM_return[simp]: "runM (return a) nd = (nd, [], a)" unfolding runM_def return_def by simp
-lemma runM_bind: "runM (a \<bind> f) nd0 = (case runM a nd0 of (nd1, msgs1, b) \<Rightarrow> case runM (f b) nd1 of (nd2, msgs2, c) \<Rightarrow> (nd2, msgs1@msgs2, c))"
-  unfolding runM_def Action_bind_def apply (cases "a", auto)
-  by (metis (no_types, lifting) Action.case Action.exhaust case_prod_conv old.prod.exhaust)
+lemma runM_bind: "runM (a \<bind> f) nd0 = (case runM a nd0 of (nd1, msgs1, result1) \<Rightarrow> (case result1 of Exception e \<Rightarrow> (nd1, msgs1, Exception e) | Success b \<Rightarrow> (case runM (f b) nd1 of (nd2, msgs2, c) \<Rightarrow> (nd2, msgs1@msgs2, c))))"
+  unfolding Action_bind_def by auto
 
 lemma return_bind[simp]: "do { a' <- return a; f a' } = f a"
-  apply (intro runM_inject) by (simp add: runM_bind return_def)
+  apply (intro runM_inject) by (simp add: runM_bind)
 lemma bind_return[simp]: "do { a' <- f; return a' } = f"
-  apply (intro runM_inject) by (simp add: runM_bind return_def)
+proof (intro runM_inject)
+  fix nd
+  obtain nd1 msgs1 result1 where result1: "runM f nd = (nd1, msgs1, result1)" by (cases "runM f nd", blast)
+  show "runM (f \<bind> return) nd = runM f nd"
+    by (cases result1, simp_all add: runM_bind result1)
+qed
 
 lemma bind_bind_assoc[simp]:
   fixes f :: "'a Action"
@@ -38,34 +47,82 @@ proof (intro runM_inject)
   fix nd0
   show "runM ?LHS nd0 = runM ?RHS nd0"
   proof (cases "runM f nd0")
-    case fields1: (fields nd1 msgs1 b)
+    case fields1: (fields nd1 msgs1 result1)
     show ?thesis
-    proof (cases "runM (g b) nd1")
-      case fields2: (fields nd2 msgs2 c)
-      show ?thesis by (cases "runM (h c) nd2", simp add: runM_bind fields1 fields2)
+    proof (cases result1)
+      case Exception show ?thesis by (simp add: runM_bind fields1 Exception)
+    next
+      case Success1: (Success b)
+      show ?thesis
+      proof (cases "runM (g b) nd1")
+        case fields2: (fields nd2 msgs2 result2)
+        show ?thesis
+        proof (cases result2)
+          case Exception show ?thesis by (simp add: runM_bind fields1 fields2 Success1 Exception)
+        next
+          case Success2: (Success c)
+          show ?thesis
+            by (cases "runM (h c) nd2", simp add: runM_bind fields1 Success1 fields2 Success2)
+        qed
+      qed
     qed
   qed
 qed
 
-definition getNodeData :: "NodeData Action" where "getNodeData \<equiv> Action (\<lambda>nd. (nd, [], nd))"
-definition setNodeData :: "NodeData \<Rightarrow> unit Action" where "setNodeData nd \<equiv> Action (\<lambda>_. (nd, [], ()))"
+definition getNodeData :: "NodeData Action" where "getNodeData \<equiv> Action (\<lambda>nd. (nd, [], Success nd))"
+definition setNodeData :: "NodeData \<Rightarrow> unit Action" where "setNodeData nd \<equiv> Action (\<lambda>_. (nd, [], Success ()))"
 
-lemma runM_getNodeData[simp]: "runM  getNodeData      nd = (nd,  [], nd)" by (simp add: runM_def getNodeData_def)
-lemma runM_setNodeData[simp]: "runM (setNodeData nd') nd = (nd', [], ())" by (simp add: runM_def setNodeData_def)
+lemma runM_getNodeData[simp]: "runM  getNodeData      nd = (nd,  [], Success nd)" by (simp add: runM_def getNodeData_def)
+lemma runM_setNodeData[simp]: "runM (setNodeData nd') nd = (nd', [], Success ())" by (simp add: runM_def setNodeData_def)
 
 lemma runM_getNodeData_continue[simp]: "runM (do { nd' <- getNodeData; f nd' }) nd = runM (f nd) nd" by (simp add: runM_bind)
 lemma runM_setNodeData_continue[simp]: "runM (do { setNodeData nd'; f }) nd = runM f nd'" by (simp add: runM_bind)
 
 definition modifyNodeData :: "(NodeData \<Rightarrow> NodeData) \<Rightarrow> unit Action" where "modifyNodeData f = getNodeData \<bind> (setNodeData \<circ> f)"
 
-lemma runM_modifyNodeData[simp]: "runM (modifyNodeData f) nd = (f nd, [], ())" by (simp add: modifyNodeData_def runM_bind)
+lemma runM_modifyNodeData[simp]: "runM (modifyNodeData f) nd = (f nd, [], Success ())" by (simp add: modifyNodeData_def runM_bind)
 lemma runM_modifyNodeData_continue[simp]: "runM (do { modifyNodeData f; a }) nd = runM a (f nd)" by (simp add: runM_bind)
 
-definition tell :: "RoutedMessage list \<Rightarrow> unit Action" where "tell rms \<equiv> Action (\<lambda>nd. (nd, rms, ()))"
-lemma runM_tell[simp]: "runM (tell rms) nd = (nd, rms, ())" by (simp add: runM_def tell_def)
+definition tell :: "RoutedMessage list \<Rightarrow> unit Action" where "tell rms \<equiv> Action (\<lambda>nd. (nd, rms, Success ()))"
+lemma runM_tell[simp]: "runM (tell rms) nd = (nd, rms, Success ())" by (simp add: runM_def tell_def)
 lemma runM_tell_contiue[simp]: "runM (do { tell rms; a }) nd = (let (nd, rms', x) = runM a nd in (nd, rms@rms', x))" by (simp add: runM_bind tell_def)
 
 definition send :: "RoutedMessage \<Rightarrow> unit Action" where "send rm = tell [rm]"
+
+definition throw :: "Exception \<Rightarrow> 'a Action" where "throw e = Action (\<lambda>nd. (nd, [], Exception e))"
+lemma runM_throw[simp]: "runM (throw e) nd = (nd, [], Exception e)" by (simp add: runM_def throw_def)
+lemma throw_continue[simp]: "do { throw e; a } = throw e" by (intro runM_inject, simp add: runM_bind)
+
+definition catch :: "'a Action \<Rightarrow> (Exception \<Rightarrow> 'a Action) \<Rightarrow> 'a Action"
+  where "catch go onException = Action (\<lambda>nd0. case runM go nd0 of (nd1, rms1, result1) \<Rightarrow> (case result1 of Success _ \<Rightarrow> (nd1, rms1, result1) | Exception e \<Rightarrow> runM (tell rms1 \<then> onException e) nd1))"
+lemma catch_throw[simp]: "catch (throw e) handle = handle e" by (intro runM_inject, simp add: catch_def)
+lemma catch_return[simp]: "catch (return a) handle = return a" by (intro runM_inject, simp add: catch_def)
+
+lemma catch_getNodeData[simp]: "catch getNodeData handle = getNodeData" by (intro runM_inject, simp add: catch_def)
+lemma catch_getNodeData_continue[simp]: "catch (do { nd <- getNodeData; f nd }) handle = do { nd <- getNodeData; catch (f nd) handle }" by (intro runM_inject, simp add: catch_def)
+lemma catch_setNodeData[simp]: "catch (setNodeData nd) handle = setNodeData nd" by (intro runM_inject, simp add: catch_def)
+lemma catch_setNodeData_continue[simp]: "catch (do { setNodeData nd; f }) handle = do { setNodeData nd; catch f handle }" by (intro runM_inject, simp add: catch_def)
+lemma catch_modifyNodeData[simp]: "catch (modifyNodeData f) handle = modifyNodeData f" by (intro runM_inject, simp add: catch_def)
+lemma catch_modifyNodeData_continue[simp]: "catch (do { modifyNodeData f; g }) handle = do { modifyNodeData f; catch g handle }" by (intro runM_inject, simp add: catch_def)
+lemma catch_tell[simp]: "catch (tell rms) handle = tell rms" by (intro runM_inject, simp add: catch_def)
+lemma catch_tell_continue[simp]: "catch (do { tell rms; f }) handle = do { tell rms; catch f handle }"
+proof (intro runM_inject)
+  fix nd0
+  show "runM (catch (do { tell rms; f }) handle) nd0 = runM (do { tell rms; catch f handle }) nd0"
+  proof (cases "runM f nd0")
+    case fields1: (fields nd1 msgs1 result1)
+    show ?thesis
+    proof (cases result1)
+      case (Exception e) show ?thesis by (cases "runM (handle e) nd1", simp add: catch_def fields1 Exception)
+    next
+      case Success1: (Success b)
+      show ?thesis
+        by (simp add: catch_def fields1 Success1)
+    qed
+  qed
+qed
+lemma catch_send[simp]: "catch (send rm) handle = send rm" by (simp add: send_def)
+lemma catch_send_continue[simp]: "catch (do { send rm; f }) handle = do { send rm; catch f handle }" by (simp add: send_def)
 
 definition gets :: "(NodeData \<Rightarrow> 'a) \<Rightarrow> 'a Action" where "gets f \<equiv> do { nd <- getNodeData; return (f nd) }"
 definition getCurrentClusterState where "getCurrentClusterState = gets currentClusterState"
@@ -101,9 +158,9 @@ definition modifyCurrentClusterState where "modifyCurrentClusterState = modifies
 definition "when" :: "bool \<Rightarrow> unit Action \<Rightarrow> unit Action" where "when c a \<equiv> if c then a else return ()"
 definition unless :: "bool \<Rightarrow> unit Action \<Rightarrow> unit Action" where "unless \<equiv> when \<circ> Not"
 
-lemma runM_when: "runM (when c a) nd = (if c then runM a nd else (nd, [], ()))"
+lemma runM_when: "runM (when c a) nd = (if c then runM a nd else (nd, [], Success ()))"
   by (auto simp add: when_def)
-lemma runM_unless: "runM (unless c a) nd = (if c then (nd, [], ()) else runM a nd)"
+lemma runM_unless: "runM (unless c a) nd = (if c then (nd, [], Success ()) else runM a nd)"
   by (auto simp add: unless_def when_def)
 
 lemma runM_when_continue: "runM (do { when c a; b }) nd = (if c then runM (do {a;b}) nd else runM b nd)"
@@ -111,15 +168,25 @@ lemma runM_when_continue: "runM (do { when c a; b }) nd = (if c then runM (do {a
 lemma runM_unless_continue: "runM (do { unless c a; b }) nd = (if c then runM b nd else runM (do {a;b}) nd)"
   by (auto simp add: unless_def when_def)
 
-definition whenCorrectDestination :: "Destination \<Rightarrow> unit Action \<Rightarrow> unit Action"
-  where "whenCorrectDestination d go \<equiv> do {
+lemma catch_when[simp]: "catch (when c a) onException = when c (catch a onException)"
+  by (intro runM_inject, simp add: catch_def runM_when)
+lemma catch_unless[simp]: "catch (unless c a) onException = unless c (catch a onException)"
+  by (intro runM_inject, simp add: catch_def runM_unless)
+
+lemma catch_when_continue[simp]: "catch (do { when c a; b }) onException = (if c then catch (do {a;b}) onException else catch b onException)"
+  by (intro runM_inject, simp add: catch_def runM_when_continue)
+lemma catch_unless_continue[simp]: "catch (do { unless c a; b }) onException = (if c then catch b onException else catch (do {a;b}) onException)"
+  by (intro runM_inject, simp add: catch_def runM_unless_continue)
+
+definition ensureCorrectDestination :: "Destination \<Rightarrow> unit Action"
+  where "ensureCorrectDestination d \<equiv> do {
     n <- getCurrentNode;
-    when (d \<in> { Broadcast, OneNode n }) go
+    when (d \<notin> { Broadcast, OneNode n }) (throw IllegalArgumentException)
   }"
 
-lemma runM_whenCorrectDestination:
-  "runM (whenCorrectDestination d go) nd = (if d \<in> { Broadcast, OneNode (currentNode nd) } then runM go nd else (nd, [], ()))"
-  by (simp add: whenCorrectDestination_def getCurrentNode_def gets_def runM_when)
+lemma runM_ensureCorrectDestination_continue:
+  "runM (do { ensureCorrectDestination d; go }) nd = (if d \<in> { Broadcast, OneNode (currentNode nd) } then runM go nd else (nd, [], Exception IllegalArgumentException))"
+  by (simp add: ensureCorrectDestination_def getCurrentNode_def gets_def runM_when_continue)
 
 definition broadcast :: "Message \<Rightarrow> unit Action"
   where "broadcast msg \<equiv> do {
@@ -127,7 +194,7 @@ definition broadcast :: "Message \<Rightarrow> unit Action"
        send \<lparr> sender = n, destination = Broadcast, payload = msg \<rparr>
     }"
 
-lemma runM_broadcast[simp]: "runM (broadcast msg) nd = (nd, [\<lparr> sender = currentNode nd, destination = Broadcast, payload = msg \<rparr>], ())"
+lemma runM_broadcast[simp]: "runM (broadcast msg) nd = (nd, [\<lparr> sender = currentNode nd, destination = Broadcast, payload = msg \<rparr>], Success ())"
   by (simp add: broadcast_def getCurrentNode_def gets_def send_def)
 
 definition sendTo :: "Node \<Rightarrow> Message \<Rightarrow> unit Action"
@@ -136,8 +203,10 @@ definition sendTo :: "Node \<Rightarrow> Message \<Rightarrow> unit Action"
        send \<lparr> sender = n, destination = OneNode d, payload = msg \<rparr>
     }"
 
-lemma runM_sendTo[simp]: "runM (sendTo d msg) nd = (nd, [\<lparr> sender = currentNode nd, destination = OneNode d, payload = msg \<rparr>], ())"
+lemma runM_sendTo[simp]: "runM (sendTo d msg) nd = (nd, [\<lparr> sender = currentNode nd, destination = OneNode d, payload = msg \<rparr>], Success ())"
   by (simp add: sendTo_def getCurrentNode_def gets_def send_def)
+
+definition ignoringExceptions :: "unit Action \<Rightarrow> unit Action" where "ignoringExceptions go \<equiv> catch go (\<lambda>_. return ())"
 
 definition getLastAcceptedTermInSlot :: "Term option Action"
   where
@@ -156,20 +225,20 @@ definition doStartJoin :: "Node \<Rightarrow> Term \<Rightarrow> unit Action"
   where
     "doStartJoin newMaster newTerm \<equiv> do {
         currentTerm <- getCurrentTerm;
-        unless (newTerm \<le> currentTerm) (do {
 
-          setJoinVotes {};
-          setElectionWon False;
-          setCurrentTerm newTerm;
-          setElectionValueForced False;
-          setPublishPermitted True;
-          setPublishVotes {};
+        when (newTerm \<le> currentTerm) (throw IllegalArgumentException);
 
-          firstUncommittedSlot <- getFirstUncommittedSlot;
-          lastAcceptedTerm <- getLastAcceptedTermInSlot;
-          sendTo newMaster (JoinRequest firstUncommittedSlot newTerm lastAcceptedTerm)
+        setCurrentTerm newTerm;
+        setJoinVotes {};
+        setElectionWon False;
+        setElectionValueForced False;
+        setPublishPermitted True;
+        setPublishVotes {};
 
-        })
+        firstUncommittedSlot <- getFirstUncommittedSlot;
+        lastAcceptedTerm <- getLastAcceptedTermInSlot;
+        sendTo newMaster (JoinRequest firstUncommittedSlot newTerm lastAcceptedTerm)
+
       }"
 
 definition doJoinRequestCurrentSlot :: "Node \<Rightarrow> Term option \<Rightarrow> unit Action"
@@ -212,16 +281,14 @@ definition doJoinRequest :: "Node \<Rightarrow> Slot \<Rightarrow> Term \<Righta
     "doJoinRequest s i t a \<equiv> do {
 
       firstUncommittedSlot <- getFirstUncommittedSlot;
-      unless (firstUncommittedSlot < i) (do {
+      when (i > firstUncommittedSlot) (throw IllegalArgumentException);
 
-        currentTerm <- getCurrentTerm;
-        when (t = currentTerm) (do {
+      currentTerm <- getCurrentTerm;
+      when (t \<noteq> currentTerm) (throw IllegalArgumentException);
 
-          if i = firstUncommittedSlot
-            then doJoinRequestCurrentSlot s a
-            else doJoinRequestCurrentSlot s None
-        })
-      })
+      if i = firstUncommittedSlot
+        then doJoinRequestCurrentSlot s a
+        else doJoinRequestCurrentSlot s None
     }"
 
 definition doClientValue :: "Value \<Rightarrow> unit Action"
@@ -229,22 +296,19 @@ definition doClientValue :: "Value \<Rightarrow> unit Action"
     "doClientValue x \<equiv> do {
 
       electionWon <- getElectionWon;
-      when electionWon (do {
+      when (\<not> electionWon) (throw IllegalArgumentException);
 
-        publishPermitted <- getPublishPermitted;
-        when publishPermitted (do {
+      publishPermitted <- getPublishPermitted;
+      when (\<not> publishPermitted) (throw IllegalArgumentException);
 
-          electionValueForced <- getElectionValueForced;
-          unless electionValueForced (do {
+      electionValueForced <- getElectionValueForced;
+      when electionValueForced (throw IllegalArgumentException);
 
-            setPublishPermitted False;
+      setPublishPermitted False;
 
-            currentTerm <- getCurrentTerm;
-            firstUncommittedSlot <- getFirstUncommittedSlot;
-            broadcast (PublishRequest firstUncommittedSlot currentTerm x)
-          })
-        })
-      })
+      currentTerm <- getCurrentTerm;
+      firstUncommittedSlot <- getFirstUncommittedSlot;
+      broadcast (PublishRequest firstUncommittedSlot currentTerm x)
     }"
 
 definition doPublishRequest :: "Node \<Rightarrow> Slot \<Rightarrow> Term \<Rightarrow> Value \<Rightarrow> unit Action"
@@ -252,15 +316,13 @@ definition doPublishRequest :: "Node \<Rightarrow> Slot \<Rightarrow> Term \<Rig
     "doPublishRequest s i t x \<equiv> do {
 
       firstUncommittedSlot <- getFirstUncommittedSlot;
-      when (i = firstUncommittedSlot) (do {
+      when (i \<noteq> firstUncommittedSlot) (throw IllegalArgumentException);
 
-        currentTerm <- getCurrentTerm;
-        when (t = currentTerm) (do {
+      currentTerm <- getCurrentTerm;
+      when (t \<noteq> currentTerm) (throw IllegalArgumentException);
 
-          setLastAcceptedData (Some \<lparr> ladSlot = i, ladTerm = t, ladValue = x \<rparr>);
-          sendTo s (PublishResponse i t)
-        })
-      })
+      setLastAcceptedData (Some \<lparr> ladSlot = i, ladTerm = t, ladValue = x \<rparr>);
+      sendTo s (PublishResponse i t)
     }"
 
 definition doPublishResponse :: "Node \<Rightarrow> Slot \<Rightarrow> Term \<Rightarrow> unit Action"
@@ -268,22 +330,19 @@ definition doPublishResponse :: "Node \<Rightarrow> Slot \<Rightarrow> Term \<Ri
     "doPublishResponse s i t \<equiv> do {
 
       firstUncommittedSlot <- getFirstUncommittedSlot;
-      when (i = firstUncommittedSlot) (do {
+      when (i \<noteq> firstUncommittedSlot) (throw IllegalArgumentException);
 
-        currentTerm <- getCurrentTerm;
-        when (t = currentTerm) (do {
+      currentTerm <- getCurrentTerm;
+      when (t \<noteq> currentTerm) (throw IllegalArgumentException);
 
-          currentVotingNodes <- getCurrentVotingNodes;
-          when (s \<in> currentVotingNodes) (do {
+      currentVotingNodes <- getCurrentVotingNodes;
+      when (s \<notin> currentVotingNodes) (throw IllegalArgumentException);
 
-            modifyPublishVotes (insert s);
-            publishVotes <- getPublishVotes;
-            currentVotingNodes <- getCurrentVotingNodes;
-            when (card publishVotes * 2 > card currentVotingNodes)
-              (broadcast (ApplyCommit i t))
-          })
-        })
-      })
+      modifyPublishVotes (insert s);
+      publishVotes <- getPublishVotes;
+      currentVotingNodes <- getCurrentVotingNodes;
+      when (card publishVotes * 2 > card currentVotingNodes)
+        (broadcast (ApplyCommit i t))
     }"
 
 definition doApplyCommit :: "Slot \<Rightarrow> Term \<Rightarrow> unit Action"
@@ -291,28 +350,26 @@ definition doApplyCommit :: "Slot \<Rightarrow> Term \<Rightarrow> unit Action"
     "doApplyCommit i t \<equiv> do {
 
       firstUncommittedSlot <- getFirstUncommittedSlot;
-      when (i = firstUncommittedSlot) (do {
+      when (i \<noteq> firstUncommittedSlot) (throw IllegalArgumentException);
 
-        lastAcceptedTerm <- getLastAcceptedTermInSlot;
-        when (Some t = lastAcceptedTerm) (do {
+      lastAcceptedTerm <- getLastAcceptedTermInSlot;
+      when (Some t \<noteq> lastAcceptedTerm) (throw IllegalArgumentException);
 
-          lastAcceptedValue <- gets lastAcceptedValue;  (* NB must be not None since electionValueForced *)
-          (case lastAcceptedValue of
-            ClusterStateDiff diff
-                \<Rightarrow> modifyCurrentClusterState diff
-            | Reconfigure votingNodes \<Rightarrow> do {
-                   setCurrentVotingNodes (set votingNodes);
-                   joinVotes <- getJoinVotes;
-                   setElectionWon (card (joinVotes \<inter> (set votingNodes)) * 2 > card (set votingNodes))
-                 }
-            | NoOp \<Rightarrow> return ());
+      lastAcceptedValue <- gets lastAcceptedValue;  (* NB must be not None since electionValueForced *)
+      (case lastAcceptedValue of
+        ClusterStateDiff diff
+            \<Rightarrow> modifyCurrentClusterState diff
+        | Reconfigure votingNodes \<Rightarrow> do {
+               setCurrentVotingNodes (set votingNodes);
+               joinVotes <- getJoinVotes;
+               setElectionWon (card (joinVotes \<inter> (set votingNodes)) * 2 > card (set votingNodes))
+             }
+        | NoOp \<Rightarrow> return ());
 
-          setFirstUncommittedSlot (i + 1);
-          setPublishPermitted True;
-          setElectionValueForced False;
-          setPublishVotes {}
-        })
-      })
+      setFirstUncommittedSlot (i + 1);
+      setPublishPermitted True;
+      setElectionValueForced False;
+      setPublishVotes {}
     }"
 
 definition doCatchUpRequest :: "Node \<Rightarrow> unit Action"
@@ -331,17 +388,16 @@ definition doCatchUpResponse :: "Slot \<Rightarrow> Node set \<Rightarrow> Clust
     "doCatchUpResponse i conf cs \<equiv> do {
 
       firstUncommittedSlot <- getFirstUncommittedSlot;
-      unless (i \<le> firstUncommittedSlot) (do {
+      when (i \<le> firstUncommittedSlot) (throw IllegalArgumentException);
 
-        setFirstUncommittedSlot i;
-        setPublishPermitted False;
-        setElectionValueForced False;
-        setPublishVotes {};
-        setCurrentVotingNodes conf;
-        setCurrentClusterState cs;
-        setJoinVotes {};
-        setElectionWon False
-      })
+      setFirstUncommittedSlot i;
+      setPublishPermitted False;
+      setElectionValueForced False;
+      setPublishVotes {};
+      setCurrentVotingNodes conf;
+      setCurrentClusterState cs;
+      setJoinVotes {};
+      setElectionWon False
     }"
 
 definition doReboot :: "unit Action"
@@ -360,10 +416,10 @@ definition doReboot :: "unit Action"
                   , publishVotes = {} \<rparr>)"
 
 definition ProcessMessageAction :: "RoutedMessage \<Rightarrow> unit Action"
-  where "ProcessMessageAction rm \<equiv> Action (\<lambda>nd. case ProcessMessage nd rm of (nd', messageOption) \<Rightarrow> (nd', case messageOption of None \<Rightarrow> [] | Some m \<Rightarrow> [m], ()))"
+  where "ProcessMessageAction rm \<equiv> Action (\<lambda>nd. case ProcessMessage nd rm of (nd', messageOption) \<Rightarrow> (nd', case messageOption of None \<Rightarrow> [] | Some m \<Rightarrow> [m], Success ()))"
 
-definition dispatchMessage :: "RoutedMessage \<Rightarrow> unit Action"
-  where "dispatchMessage m \<equiv> whenCorrectDestination (destination m) (case payload m of
+definition dispatchMessageInner :: "RoutedMessage \<Rightarrow> unit Action"
+  where "dispatchMessageInner m \<equiv> case payload m of
           StartJoin t \<Rightarrow> doStartJoin (sender m) t
           | JoinRequest i t a \<Rightarrow> doJoinRequest (sender m) i t a
           | ClientValue x \<Rightarrow> doClientValue x
@@ -372,7 +428,13 @@ definition dispatchMessage :: "RoutedMessage \<Rightarrow> unit Action"
           | ApplyCommit i t \<Rightarrow> doApplyCommit i t
           | CatchUpRequest \<Rightarrow> doCatchUpRequest (sender m)
           | CatchUpResponse i conf cs \<Rightarrow> doCatchUpResponse i conf cs
-          | Reboot \<Rightarrow> doReboot)"
+          | Reboot \<Rightarrow> doReboot"
+
+definition dispatchMessage :: "RoutedMessage \<Rightarrow> unit Action"
+  where "dispatchMessage m \<equiv> ignoringExceptions (do {
+      ensureCorrectDestination (destination m);
+      dispatchMessageInner m
+    })"
 
 lemma getLastAcceptedTermInSlot_gets[simp]: "getLastAcceptedTermInSlot = gets lastAcceptedTermInSlot"
 proof (intro runM_inject)
@@ -389,17 +451,28 @@ proof (intro ext runM_inject)
   show "runM (dispatchMessage rm) nd = runM (ProcessMessageAction rm) nd" (is "?LHS = ?RHS")
   proof (cases "destination rm \<in> {Broadcast, OneNode (currentNode nd)}")
     case False
-    thus ?thesis
-      unfolding ProcessMessageAction_def dispatchMessage_def whenCorrectDestination_def getCurrentNode_def gets_def ProcessMessage_def Let_def
-      by (simp add: runM_when)
+
+    hence 1: "\<And>f. runM (do { ensureCorrectDestination (destination rm); f }) nd = (nd, [], Exception IllegalArgumentException)"
+      by (simp add: runM_ensureCorrectDestination_continue)
+
+    from False
+    show ?thesis
+      unfolding ProcessMessageAction_def dispatchMessage_def
+      by (simp add: ignoringExceptions_def catch_def 1 ProcessMessage_def)
   next
     case dest_ok: True
 
-    show ?thesis
+    hence 1: "runM (dispatchMessage rm) nd = runM (ignoringExceptions (dispatchMessageInner rm)) nd"
+      by (simp add: dispatchMessage_def ignoringExceptions_def catch_def runM_ensureCorrectDestination_continue)
+
+    also have "... = runM (ProcessMessageAction rm) nd" (is "?LHS = ?RHS")
     proof (cases "payload rm")
       case (StartJoin t)
 
-      consider
+      have "?LHS = runM (ignoringExceptions (doStartJoin (sender rm) t)) nd" (is "_ = ?STEP")
+        by (simp add: dispatchMessageInner_def StartJoin)
+
+      also consider
         (a) "t \<le> currentTerm nd"
         | (b) "currentTerm nd < t" "case lastAcceptedTerm nd of None \<Rightarrow> False | Some x \<Rightarrow> t \<le> x"
         | (c) "currentTerm nd < t" "case lastAcceptedTerm nd of None \<Rightarrow> True | Some x \<Rightarrow> x < t"
@@ -411,36 +484,44 @@ proof (intro ext runM_inject)
           by (cases "case lastAcceptedTerm nd of None \<Rightarrow> False | Some x \<Rightarrow> t \<le> x", auto, cases "lastAcceptedTerm nd", auto)
       qed
 
-      thus ?thesis
+      hence "?STEP = ?RHS"
       proof cases
         case a
-        with StartJoin dest_ok show ?thesis
-          by (simp add: ProcessMessageAction_def dispatchMessage_def runM_whenCorrectDestination ProcessMessage_def Let_def runM_unless
+        thus ?thesis
+          by (simp add: StartJoin ProcessMessageAction_def dispatchMessage_def ProcessMessage_def Let_def runM_unless
               doStartJoin_def getCurrentTerm_def gets_def setJoinVotes_def sets_def setCurrentTerm_def setElectionValueForced_def
-              setPublishPermitted_def setPublishVotes_def getFirstUncommittedSlot_def handleStartJoin_def ensureCurrentTerm_def setElectionWon_def)
+              setPublishPermitted_def setPublishVotes_def getFirstUncommittedSlot_def handleStartJoin_def ensureCurrentTerm_def setElectionWon_def
+              ignoringExceptions_def catch_def runM_when_continue)
       next
         case b
         with StartJoin dest_ok show ?thesis
-          by (cases "lastAcceptedTerm nd ", simp_all add: ProcessMessageAction_def dispatchMessage_def runM_whenCorrectDestination ProcessMessage_def Let_def
+          by (cases "lastAcceptedTerm nd ", simp_all add: ProcessMessageAction_def dispatchMessage_def ProcessMessage_def Let_def
               doStartJoin_def getCurrentTerm_def gets_def setJoinVotes_def sets_def setCurrentTerm_def setElectionValueForced_def runM_unless lastAcceptedTerm_def lastAcceptedSlot_def
-              setPublishPermitted_def setPublishVotes_def getFirstUncommittedSlot_def handleStartJoin_def ensureCurrentTerm_def setElectionWon_def lastAcceptedTermInSlot_def)
+              setPublishPermitted_def setPublishVotes_def getFirstUncommittedSlot_def handleStartJoin_def ensureCurrentTerm_def setElectionWon_def lastAcceptedTermInSlot_def
+              ignoringExceptions_def catch_def runM_when_continue)
       next
         case c with StartJoin dest_ok show ?thesis
-          by (cases "lastAcceptedTerm nd", simp_all add: ProcessMessageAction_def dispatchMessage_def runM_whenCorrectDestination ProcessMessage_def Let_def
+          by (cases "lastAcceptedTerm nd", simp_all add: ProcessMessageAction_def dispatchMessage_def ProcessMessage_def Let_def
               doStartJoin_def getCurrentTerm_def gets_def setJoinVotes_def sets_def setCurrentTerm_def setElectionValueForced_def runM_unless lastAcceptedTerm_def lastAcceptedSlot_def
-              setPublishPermitted_def setPublishVotes_def getFirstUncommittedSlot_def handleStartJoin_def ensureCurrentTerm_def setElectionWon_def lastAcceptedTermInSlot_def)
+              setPublishPermitted_def setPublishVotes_def getFirstUncommittedSlot_def handleStartJoin_def ensureCurrentTerm_def setElectionWon_def lastAcceptedTermInSlot_def
+              ignoringExceptions_def catch_def runM_when_continue)
       qed
+
+      finally show ?thesis by simp
 
     next
       case (JoinRequest i t a)
 
-      show ?thesis
+      have "?LHS = runM (ignoringExceptions (doJoinRequest (sender rm) i t a)) nd" (is "_ = ?STEP")
+        by (simp add: dispatchMessageInner_def JoinRequest)
+
+      also have "... = ?RHS"
       proof (cases "firstUncommittedSlot nd < i")
         case True
         with JoinRequest dest_ok show ?thesis
-          by (simp add: dispatchMessage_def runM_whenCorrectDestination runM_unless
+          by (simp add: dispatchMessage_def runM_unless
               doJoinRequest_def gets_def getFirstUncommittedSlot_def ProcessMessage_def
-              ProcessMessageAction_def handleJoinRequest_def)
+              ProcessMessageAction_def handleJoinRequest_def ignoringExceptions_def)
       next
         case False hence le: "i \<le> firstUncommittedSlot nd" by simp
 
@@ -448,9 +529,9 @@ proof (intro ext runM_inject)
         proof (cases "t = currentTerm nd")
           case False
           with JoinRequest dest_ok le show ?thesis
-            by (simp add: dispatchMessage_def runM_whenCorrectDestination runM_when runM_unless
+            by (simp add: dispatchMessage_def runM_when runM_unless
                 doJoinRequest_def gets_def getFirstUncommittedSlot_def getCurrentTerm_def
-                ProcessMessage_def ProcessMessageAction_def handleJoinRequest_def)
+                ProcessMessage_def ProcessMessageAction_def handleJoinRequest_def ignoringExceptions_def)
 
         next
           case t: True
@@ -459,24 +540,24 @@ proof (intro ext runM_inject)
           proof (cases "i = firstUncommittedSlot nd")
             case False
             with JoinRequest dest_ok le t show ?thesis
-              by (simp add: dispatchMessage_def runM_whenCorrectDestination Let_def runM_when_continue
+              by (simp add: dispatchMessage_def Let_def runM_when_continue
                 doJoinRequest_def doJoinRequestCurrentSlot_def runM_when runM_unless
                 gets_def getFirstUncommittedSlot_def getCurrentTerm_def
                 getElectionValueForced_def getJoinVotes_def getCurrentVotingNodes_def
-                getPublishPermitted_def
-                modifies_def modifyJoinVotes_def
+                getPublishPermitted_def ignoringExceptions_def broadcast_def getCurrentNode_def
+                modifies_def modifyJoinVotes_def send_def
                 sets_def setElectionWon_def setPublishPermitted_def lastAcceptedValue_def
                 ProcessMessage_def ProcessMessageAction_def handleJoinRequest_def
                 addElectionVote_def publishValue_def isQuorum_def majorities_def)
           next
             case True
             with JoinRequest dest_ok le t show ?thesis
-              by (simp add: dispatchMessage_def runM_whenCorrectDestination Let_def
+              by (simp add: dispatchMessage_def Let_def
                   doJoinRequest_def doJoinRequestCurrentSlot_def
                   runM_unless runM_when runM_when_continue
                   gets_def getFirstUncommittedSlot_def getCurrentTerm_def
                   getElectionValueForced_def getJoinVotes_def getCurrentVotingNodes_def
-                  getPublishPermitted_def
+                  getPublishPermitted_def send_def broadcast_def ignoringExceptions_def catch_def getCurrentNode_def
                   modifies_def modifyJoinVotes_def lastAcceptedValue_def
                   sets_def setElectionWon_def setPublishPermitted_def setElectionValueForced_def
                   ProcessMessage_def ProcessMessageAction_def handleJoinRequest_def
@@ -485,29 +566,33 @@ proof (intro ext runM_inject)
         qed
       qed
 
+      finally show ?thesis by simp
+
     next
-      case (ClientValue x) with dest_ok show ?thesis
-        by (simp add: ProcessMessageAction_def dispatchMessage_def runM_whenCorrectDestination
+      case (ClientValue x)
+
+      with dest_ok show ?thesis
+        by (simp add: ProcessMessageAction_def dispatchMessageInner_def
             doClientValue_def gets_def getElectionValueForced_def getElectionWon_def
             runM_unless getPublishPermitted_def setPublishPermitted_def sets_def
             getCurrentTerm_def getFirstUncommittedSlot_def ProcessMessage_def handleClientValue_def
-            publishValue_def runM_when)
+            publishValue_def runM_when ignoringExceptions_def ClientValue catch_def runM_when_continue)
 
     next
       case (PublishRequest i t x) with dest_ok show ?thesis
-        by (simp add: ProcessMessageAction_def dispatchMessage_def runM_whenCorrectDestination
+        by (simp add: ProcessMessageAction_def dispatchMessageInner_def
           doPublishRequest_def gets_def getCurrentTerm_def getFirstUncommittedSlot_def
-          sets_def setLastAcceptedData_def
+          sets_def setLastAcceptedData_def ignoringExceptions_def catch_def runM_when_continue
           getCurrentNode_def runM_unless send_def
           ProcessMessage_def handlePublishRequest_def runM_when)
 
     next
       case (PublishResponse i t) with dest_ok show ?thesis
-        by (simp add: ProcessMessageAction_def dispatchMessage_def runM_whenCorrectDestination
+        by (simp add: ProcessMessageAction_def dispatchMessageInner_def
           doPublishResponse_def gets_def getCurrentTerm_def getFirstUncommittedSlot_def
           broadcast_def getCurrentNode_def runM_unless send_def
           modifyPublishVotes_def modifies_def getPublishVotes_def getCurrentVotingNodes_def
-          runM_when
+          runM_when ignoringExceptions_def catch_def runM_when_continue
           ProcessMessage_def handlePublishResponse_def commitIfQuorate_def isQuorum_def majorities_def)
 
     next
@@ -517,60 +602,66 @@ proof (intro ext runM_inject)
       proof (cases "lastAcceptedValue nd")
         case NoOp
         with ApplyCommit dest_ok show ?thesis
-          by (simp add: ProcessMessageAction_def dispatchMessage_def runM_whenCorrectDestination
+          by (simp add: ProcessMessageAction_def dispatchMessageInner_def
             doApplyCommit_def runM_unless runM_when
             gets_def getFirstUncommittedSlot_def
             sets_def setFirstUncommittedSlot_def
             setPublishPermitted_def setElectionValueForced_def setPublishVotes_def
-            ProcessMessage_def handleApplyCommit_def applyAcceptedValue_def)
+            ProcessMessage_def handleApplyCommit_def applyAcceptedValue_def
+            ignoringExceptions_def catch_def runM_when_continue)
       next
         case Reconfigure
         with ApplyCommit dest_ok show ?thesis
-          by (simp add: ProcessMessageAction_def dispatchMessage_def runM_whenCorrectDestination
+          by (simp add: ProcessMessageAction_def dispatchMessageInner_def
             doApplyCommit_def runM_unless runM_when
             gets_def getFirstUncommittedSlot_def
             getJoinVotes_def
             sets_def setFirstUncommittedSlot_def
             setPublishPermitted_def setElectionValueForced_def setPublishVotes_def
             setCurrentVotingNodes_def setElectionWon_def
-            ProcessMessage_def handleApplyCommit_def applyAcceptedValue_def majorities_def)
+            ProcessMessage_def handleApplyCommit_def applyAcceptedValue_def majorities_def
+            ignoringExceptions_def catch_def runM_when_continue)
       next
         case ClusterStateDiff
         with ApplyCommit dest_ok show ?thesis
-          by (simp add: ProcessMessageAction_def dispatchMessage_def runM_whenCorrectDestination
+          by (simp add: ProcessMessageAction_def dispatchMessageInner_def
             doApplyCommit_def runM_unless runM_when
             gets_def getFirstUncommittedSlot_def
             sets_def setFirstUncommittedSlot_def
             modifies_def modifyCurrentClusterState_def
             setPublishPermitted_def setElectionValueForced_def setPublishVotes_def
-            ProcessMessage_def handleApplyCommit_def applyAcceptedValue_def)
+            ProcessMessage_def handleApplyCommit_def applyAcceptedValue_def
+            ignoringExceptions_def catch_def runM_when_continue)
       qed
 
     next
       case CatchUpRequest
       with dest_ok show ?thesis
-        by (simp add: ProcessMessageAction_def dispatchMessage_def runM_whenCorrectDestination
+        by (simp add: ProcessMessageAction_def dispatchMessageInner_def
           doCatchUpRequest_def
           gets_def getFirstUncommittedSlot_def getCurrentVotingNodes_def getCurrentClusterState_def
-          ProcessMessage_def handleCatchUpRequest_def)
+          ProcessMessage_def handleCatchUpRequest_def ignoringExceptions_def catch_def runM_when_continue)
 
     next
       case (CatchUpResponse i conf cs)
       with dest_ok show ?thesis
-        by (simp add: ProcessMessageAction_def dispatchMessage_def runM_whenCorrectDestination
+        by (simp add: ProcessMessageAction_def dispatchMessageInner_def
             doCatchUpResponse_def gets_def getFirstUncommittedSlot_def
             sets_def setFirstUncommittedSlot_def
             setPublishPermitted_def setElectionValueForced_def setPublishVotes_def
             setCurrentVotingNodes_def setCurrentClusterState_def setJoinVotes_def
             setElectionWon_def runM_unless
-            ProcessMessage_def handleCatchUpResponse_def)
+            ProcessMessage_def handleCatchUpResponse_def
+            ignoringExceptions_def catch_def runM_when_continue)
 
     next
       case Reboot
       with dest_ok show ?thesis
-        by (simp add: ProcessMessageAction_def dispatchMessage_def runM_whenCorrectDestination
-          doReboot_def ProcessMessage_def handleReboot_def)
+        by (simp add: ProcessMessageAction_def dispatchMessageInner_def
+            doReboot_def ProcessMessage_def handleReboot_def ignoringExceptions_def catch_def runM_when_continue)
     qed
+
+    finally show ?thesis .
   qed
 qed
 
